ITree_Deadlock.thy
@@ -1,0 +1,18 @@
+section \<open> Deadlock \<close>
+
+theory ITree_Deadlock
+  imports ITree_Divergence
+begin
+
+text \<open> Deadlock is an interaction with no visible event \<close>
+
+definition deadlock :: "('e, 'r) itree" where
+"deadlock = Vis [\<mapsto>]"
+
+lemma deadlock_trace_to: "deadlock \<midarrow>tr\<leadsto> P \<longleftrightarrow> tr = [] \<and> P = deadlock"
+  by (metis deadlock_def domIff trace_to_Nil trace_to_VisE)
+
+definition deadlock_free :: "('e, 'r) itree \<Rightarrow> bool" where
+"deadlock_free P = (\<forall> tr. \<not> P \<midarrow>tr\<leadsto> deadlock)"
+
+end
